Term_equality.v
@@ -17,8 +17,8 @@ Notation terms := (vector term).
 
 CoInductive term_bis : term -> term -> Prop :=
   | Var_bis : forall x, term_bis (Var x) (Var x)
-  | Fun_bis : forall f v w, 
-              (forall i, term_bis (v i) (w i)) -> 
+  | Fun_bis : forall f v w,
+              (forall i, term_bis (v i) (w i)) ->
               term_bis (Fun f v) (Fun f w).
 
 (* Equality of infinite terms up to a given depth *)
@@ -26,14 +26,14 @@ CoInductive term_bis : term -> term -> Prop :=
 Inductive term_eq_up_to : nat -> term -> term -> Prop :=
   | teut_0   : forall t u : term, term_eq_up_to 0 t u
   | teut_var : forall n x, term_eq_up_to n (Var x) (Var x)
-  | teut_fun : forall n f v w, 
-               (forall i, term_eq_up_to n (v i) (w i)) -> 
+  | teut_fun : forall n f v w,
+               (forall i, term_eq_up_to n (v i) (w i)) ->
                term_eq_up_to (S n) (Fun f v) (Fun f w).
 
-Definition term_eq (t u : term) := 
+Definition term_eq (t u : term) :=
   forall n, term_eq_up_to n t u.
 
-(* We do not see how to prove the following lemma without appeal to JMeq 
+(* We do not see how to prove the following lemma without appeal to JMeq
    (as used by the tactic [dependent destruction]):
 *)
 
@@ -54,7 +54,7 @@ intros f v w H i n.
 apply teut_fun_inv with (1 := H (S n)).
 Qed.
 
-Lemma term_bis_implies_term_eq : 
+Lemma term_bis_implies_term_eq :
   forall (t u : term), term_bis t u -> term_eq t u.
 Proof.
 intros t u H n.
@@ -68,7 +68,7 @@ intro i.
 apply IHn with (1:=(H i)).
 Qed.
 
-Lemma term_eq_fun_inv_symbol : 
+Lemma term_eq_fun_inv_symbol :
   forall (f g : F) (v : terms (arity f)) (w : terms (arity g)),
   term_eq (Fun f v) (Fun g w) -> f = g.
 Proof.
@@ -94,6 +94,39 @@ assert (H0 := term_eq_fun_inv H).
 apply eq2bis.
 apply H0.
 Qed.
+
+Lemma term_eq_refl : forall t, term_eq t t.
+Proof.
+intros t n.
+generalize t. clear t.
+induction n as [| n IH]; intro t.
+constructor.
+destruct t.
+constructor.
+constructor.
+intro.
+apply IH.
+Qed.
+
+Lemma term_eq_symm : forall t u, term_eq t u -> term_eq u t.
+Proof.
+intros t u H n.
+assert (H0 := H n). clear H.
+generalize t u H0. clear H0 u t.
+induction n; intros.
+constructor.
+inversion H0.
+constructor.
+constructor.
+intro.
+apply IHn.
+apply H1.
+Qed.
+
+(* TODO
+Lemma term_eq_trans : forall t u v, term_eq t u -> term_eq u v -> term_eq t v.
+Proof.
+*)
 
 Lemma term_bis_refl : forall t, term_bis t t.
 cofix.
@@ -129,5 +162,3 @@ End term_equality.
 
 Infix " [~] " := term_bis (no associativity, at level 70).
 Infix " [=] " := term_eq (no associativity, at level 70).
-
-
